Add proof producing procedures for naive ijr transformation and contract transfer (#9)
* Add definitions of resolve_fully and resolve_fully_n and necessary theorems, in particular, contract transfer theorem
* Add proof producing procedures for resolve_fully_n and contract transfer
* Remove unnecessary assumption from resolved and change ending statement on resolved_fail
* Add examples for resolve_fully, resolve_fully_n and proof producing procedures

examples/ijr/resolveFullyLib.sml
@@ -1,0 +1,38 @@
+structure resolveFullyLib =
+struct
+open HolKernel Parse boolLib bossLib;
+
+open optionSyntax bir_htSyntax;
+
+open resolveFullyTheory;
+
+fun resolve_indirect_jumps(prog_tm, args) =
+  let
+    val prog'_thm = EVAL “resolve_fully_n ^prog_tm ^args”
+    val prog'_tm = (dest_some o rhs o concl) prog'_thm
+    val prog'_var = mk_var("prog'", type_of prog'_tm)
+    val prog'_def = Define `^prog'_var = ^prog'_tm`
+    val prog'_tm' = (lhs o concl) prog'_def
+    val prog'_thm' = REWRITE_RULE [GSYM prog'_def] prog'_thm
+  in
+    (prog'_tm', prog'_def, prog'_thm')
+  end
+
+fun transfer_contract(prog_tm, prog'_thm, ht_thm) =
+  let
+    val ht_tm = concl ht_thm
+    val (_, entry_tm, exits_tm, _, _) = dest_bir_exec_to_labels_triple ht_tm
+    val entry_thm = prove (
+      “MEM ^entry_tm (bir_labels_of_program ^prog_tm)”,
+      EVAL_TAC)
+    val ending_thm = prove (
+      “^exits_tm SUBSET (set (bir_labels_of_program ^prog_tm))”,
+      EVAL_TAC)
+    val res_thm = MATCH_MP resolve_fully_n_contract_transfer prog'_thm
+    val res_thm = MATCH_MP res_thm entry_thm
+    val res_thm = MATCH_MP res_thm ending_thm
+  in
+    MATCH_MP res_thm ht_thm
+  end
+
+end
