examples/ijr/examplesScript.sml
@@ -1,11 +1,17 @@
 open HolKernel Parse boolLib bossLib;
 
-open bslSyntax bir_execLib;
+open bslSyntax bir_execLib bir_bool_expTheory bir_htSyntax;
+open bir_wp_interfaceLib;
+open tutorial_smtSupportLib;
+open bir_compositionLib;
 
-open resolveTheory;
+open resolveTheory resolveFullyTheory;
+open resolveFullyLib;
 
 val _ = new_theory "examples";
 
+
+val _ = bir_ppLib.install_bir_pretty_printers();
 
 val observe_type = Type `: 'a`
 val bdefprog_list = bdefprog_list observe_type
@@ -14,23 +20,103 @@ val block1 = (blabel_addr32 0,
               [bassign (bvarimm32 "y", bconst32 4)],
               (bjmp o belabel_expr o bden o bvarimm32) "y")
 
-val block2: term * term list * term  = (blabel_addr32 4, [], (bhalt o bconst32) 0)
+val block2: term * term list * term  = (blabel_addr32 4,
+                                        [],
+                                        (bhalt o bconst32) 0)
 
+
+(*Program definition*)
 val prog_def = bdefprog_list "prog" [block1, block2]
-val prog = (snd o dest_eq o concl) prog_def
+val prog_tm = (rhs o concl) prog_def
+(*val _ = bir_exec_prog_print "prog" prog_tm 10 NONE NONE NONE;*)
 
-val n_max = 10;
-val _ = bir_exec_prog_print "prog" prog n_max NONE NONE NONE;
+val prog_var = mk_var("prog", type_of prog_tm);
+val prog_def = Define `^prog_var = ^prog_tm`;
+val prog_tm' = (lhs o concl) prog_def
 
-val prog'_def = EVAL “resolve_fail ^prog (BL_Address (Imm32 0w))”
-val prog' = (dest_some o snd o dest_eq o concl) prog'_def
 
-val _ = bir_exec_prog_print "prog'" prog' n_max NONE NONE NONE;
+(*resolve_fail and resolve tests*)
+val prog'_thm = EVAL “resolve_fail ^prog_tm (BL_Address (Imm32 0w)) (Imm32 4w)”
+val prog'_tm = (dest_some o rhs o concl) prog'_thm
+(*val _ = bir_exec_prog_print "prog'" prog'_tm 10 NONE NONE NONE;*)
 
-val prog'_def = EVAL “resolve ^prog (BL_Address (Imm32 0w)) (Imm32 10w) "fresh"”
-val prog' = (dest_some o snd o dest_eq o concl) prog'_def
-
+val prog'_thm = EVAL “resolve ^prog_tm (BL_Address (Imm32 0w)) (Imm32 10w) "0w-1"”
+val prog'_tm = (dest_some o rhs o concl) prog'_thm
 (*val _ = bir_exec_prog_print "prog'" prog' n_max NONE NONE NONE;*)
+
+
+(*resolve_fully test*)
+val arg1 = “BL_Address (Imm32 0w)”
+val arg2 = “[(Imm32 10w, "0w-1"); (Imm32 4w, "0w-2")]”
+val arg3 = “Imm32 4w”
+val prog'_thm = EVAL “resolve_fully ^prog_tm ^arg1 ^arg2 ^arg3”
+val prog'_tm = (dest_some o rhs o concl) prog'_thm
+
+
+(*resolve_fully_n one indirect jump test many steps*)
+val args = “[(^arg1, ^arg2, ^arg3)]”
+val prog'_thm = EVAL “resolve_fully_n ^prog_tm ^args”
+val prog'_tm = (dest_some o rhs o concl) prog'_thm
+
+
+(*resolve_fully_n many indirect jumps many steps test*)
+val block1' = (blabel_addr32 8,
+               [bassign (bvarimm32 "z", bconst32 4)],
+               (bjmp o belabel_expr o bden o bvarimm32) "z")
+val prog2_def = bdefprog_list "prog2" [block1, block2, block1']
+val prog2_tm = (rhs o concl) prog2_def
+
+val args = “[(^arg1, ^arg2, ^arg3);
+             (BL_Address (Imm32 8w), [(Imm32 10w, "8w-1"); (Imm32 4w, "8w-2")], ^arg3)]”
+val prog2'_thm = EVAL “resolve_fully_n ^prog2_tm ^args”
+val prog2'_tm = (dest_some o rhs o concl) prog2'_thm
+
+
+(*contract transfer test*)
+(*Transform program*)
+val args = “[(BL_Address (Imm32 0w), [(Imm32 4w, "0w-2")], ^arg3)]”
+val (prog'_tm, prog'_def, prog'_thm) = resolve_indirect_jumps(prog_tm', args)
+
+(*Obtain WP contract*)
+val pre_def = Define ‘pre = bir_exp_true’;
+val post_def = Define ‘post = ^(beq((bden o bvarimm32) "y", bconst32 4))’;
+
+val prefix = "example_";
+val entry_label_tm = “BL_Address (Imm32 0w)”;
+val ending_labels_tm = “{BL_Address (Imm32 4w)}”;
+val post_tm = “\l. if (l = BL_Address (Imm32 4w))
+                   then post
+                   else bir_exp_false”;
+val defs = [prog'_def, post_def, bir_exp_false_def];
+
+val (ht_thm, wp_tm) =
+  bir_obtain_ht prog'_tm entry_label_tm
+                ending_labels_tm ending_set_to_sml_list
+                post_tm postcond_exp_from_label
+                prefix defs;
+
+val wp_def = Define `wp = ^(wp_tm)`;
+val ht_thm' = REWRITE_RULE [GSYM wp_def] ht_thm;
+
+(*
+val defs = [prog_def, post_def, bir_exp_true_def, bir_exp_false_def];
+val (ht, wp_tm) =
+  bir_obtain_ht prog_tm entry_label_tm
+                ending_labels_tm ending_set_to_sml_list
+                post_tm postcond_exp_from_label
+                prefix defs;
+*)
+
+(*Transfer WP contract*)
+val ht'_thm = transfer_contract(prog_tm', prog'_thm, ht_thm')
+
+(*Obtain contract by proving implication*)
+val contract_pre = (lhs o concl) pre_def;
+val contract_wp = (lhs o concl) wp_def;
+val contract_imp = bimp (contract_pre, contract_wp);
+val contract_imp_taut_thm = prove_exp_is_taut contract_imp;
+val contract =
+  label_ct_to_simp_ct_predset ht'_thm contract_imp_taut_thm;
 
 
 val _ = export_theory();
