examples/ijr/resolveFullyScript.sml
@@ -1,0 +1,188 @@
+open HolKernel Parse boolLib bossLib;
+
+open listTheory optionTheory pred_setTheory pred_setSimps;
+
+open bir_programTheory bir_program_blocksTheory;
+open HolBACoreSimps;
+
+open resolutionTheory resolveTheory contractTransferTheory;
+
+val _ = new_theory "resolveFully";
+
+
+Definition direct_jump_targets_block_compute_def:
+  direct_jump_targets_block_compute bl =
+  case bl.bb_last_statement of
+    BStmt_Jmp (BLE_Label l) => [l]
+  | BStmt_CJmp e (BLE_Label l1) (BLE_Label l2) => [l1; l2]
+  | BStmt_CJmp e (BLE_Label l1) _ => [l1]
+  | BStmt_CJmp e  _ (BLE_Label l2) => [l2]
+  | _ => []
+End
+
+Theorem direct_jump_target_block_direct_jump_targets_block_compute:
+  ∀l bl.
+    direct_jump_target_block l bl ⇒
+    MEM l (direct_jump_targets_block_compute bl)
+Proof
+SIMP_TAC std_ss [direct_jump_target_block_def] >>
+REPEAT STRIP_TAC >- (
+  ASM_SIMP_TAC (list_ss++bir_TYPES_ss) [direct_jump_targets_block_compute_def]
+) >- (
+  Cases_on ‘l2’ >>
+  ASM_SIMP_TAC (list_ss++bir_TYPES_ss) [direct_jump_targets_block_compute_def]
+) >>
+Cases_on ‘l1’ >>
+ASM_SIMP_TAC (list_ss++bir_TYPES_ss) [direct_jump_targets_block_compute_def]
+QED
+
+Definition direct_jump_targets_compute_def:
+  direct_jump_targets_compute (BirProgram bls) =
+  LIST_BIND bls direct_jump_targets_block_compute
+End
+
+Theorem direct_jump_target_direct_jump_targets_compute:
+  ∀l p. direct_jump_target l p ⇒
+        MEM l (direct_jump_targets_compute p)
+Proof
+Cases_on ‘p’ >> rename1 ‘BirProgram p’ >>
+SIMP_TAC std_ss [direct_jump_target_def] >>
+REPEAT STRIP_TAC >>
+SIMP_TAC list_ss [direct_jump_targets_compute_def, LIST_BIND_def, MEM_FLAT, MEM_MAP] >>
+Q.EXISTS_TAC ‘direct_jump_targets_block_compute bl’ >>
+STRIP_TAC >- (
+  Q.EXISTS_TAC ‘bl’ >>
+  ASM_SIMP_TAC std_ss [MEM_EL] >>
+  PROVE_TAC [bir_get_program_block_info_by_label_THM, bir_get_current_block_SOME]
+) >>
+
+IMP_RES_TAC direct_jump_target_block_direct_jump_targets_block_compute
+QED
+
+Definition fresh_label_compute_def:
+  fresh_label_compute l p =
+  (~(MEM l (bir_labels_of_program p)) ∧
+   ~(MEM l (direct_jump_targets_compute p)))
+End
+
+Theorem fresh_label_compute_sound:
+  ∀l p. fresh_label_compute l p ⇒ fresh_label l p
+Proof
+SIMP_TAC std_ss [fresh_label_compute_def, fresh_label_def] >>
+REPEAT STRIP_TAC >>
+PROVE_TAC [direct_jump_target_direct_jump_targets_compute]
+QED
+
+Definition resolve_fully_def:
+  (resolve_fully p l [] v = resolve_fail p l v) ∧
+  (resolve_fully p l ((v, sl) :: xs) v' =
+     if fresh_label_compute (BL_Label sl) p then
+       OPTION_BIND (resolve p l v sl) (\p'. resolve_fully p' (BL_Label sl) xs v')
+     else NONE)
+End
+
+Theorem resolve_fully_simulated_termination:
+  ∀p l xs v' p'.
+    resolve_fully p l xs v' = SOME p' ⇒
+    simulated_termination p p'
+Proof
+Induct_on ‘xs’ >>
+REPEAT GEN_TAC >- (
+  PROVE_TAC [resolve_fully_def, resolve_fail_simulated_termination]
+) >>
+
+rename1 ‘SOME p''’ >>
+Cases_on ‘h’ >> rename1 ‘(v, sl)’ >>
+SIMP_TAC std_ss [resolve_fully_def] >>
+PROVE_TAC [resolve_simulated_termination, fresh_label_compute_sound,
+           resolve_labels, simulated_termination_transitive]
+QED
+
+Theorem resolve_fully_vars:
+  ∀p l xs v' p'.
+    resolve_fully p l xs v' = SOME p' ⇒
+    bir_vars_of_program p' SUBSET bir_vars_of_program p
+Proof
+Induct_on ‘xs’ >>
+REPEAT GEN_TAC >- (
+  PROVE_TAC [resolve_fully_def, resolve_fail_vars]
+) >>
+
+rename1 ‘SOME p''’ >>
+Cases_on ‘h’ >> rename1 ‘(v, sl)’ >>
+SIMP_TAC std_ss [resolve_fully_def] >>
+PROVE_TAC [resolve_vars, SUBSET_TRANS]
+QED
+
+Theorem resolve_fully_labels:
+  ∀p l xs v' p'.
+    resolve_fully p l xs v' = SOME p' ⇒
+    set (bir_labels_of_program p) SUBSET set (bir_labels_of_program p')
+Proof
+Induct_on ‘xs’ >>
+REPEAT GEN_TAC >- (
+  PROVE_TAC [resolve_fully_def, resolve_fail_labels, SUBSET_REFL]
+) >>
+
+rename1 ‘SOME p''’ >>
+Cases_on ‘h’ >> rename1 ‘(v, sl)’ >>
+SIMP_TAC std_ss [resolve_fully_def] >>
+PROVE_TAC [resolve_labels, SUBSET_TRANS]
+QED
+
+Definition resolve_fully_n_def:
+  (resolve_fully_n p [] = SOME p) ∧
+  (resolve_fully_n p ((l, xs, v) :: ys) =
+     OPTION_BIND (resolve_fully p l xs v) (\p'. resolve_fully_n p' ys))
+End
+
+Theorem resolve_fully_n_simulated_termination:
+  ∀p ys p'.
+    resolve_fully_n p ys = SOME p' ⇒
+    simulated_termination p p'
+Proof
+Induct_on ‘ys’ >>
+REPEAT GEN_TAC >- (
+  SIMP_TAC std_ss [resolve_fully_n_def, simulated_termination_REFL]
+) >>
+
+rename1 ‘SOME p''’ >>
+Cases_on ‘h’ >> Cases_on ‘r’ >> rename1 ‘(l, xs, v)’ >>
+SIMP_TAC std_ss [resolve_fully_n_def] >>
+PROVE_TAC [resolve_fully_simulated_termination,
+           resolve_fully_labels, simulated_termination_transitive]
+QED
+
+Theorem resolve_fully_n_vars:
+  ∀p ys p'.
+    resolve_fully_n p ys = SOME p' ⇒
+    bir_vars_of_program p' SUBSET bir_vars_of_program p
+Proof
+Induct_on ‘ys’ >>
+REPEAT GEN_TAC >- (
+  SIMP_TAC std_ss [resolve_fully_n_def, SUBSET_REFL]
+) >>
+
+rename1 ‘SOME p''’ >>
+Cases_on ‘h’ >> Cases_on ‘r’ >> rename1 ‘(l, xs, v)’ >>
+SIMP_TAC std_ss [resolve_fully_n_def] >>
+PROVE_TAC [resolve_fully_vars, SUBSET_TRANS]
+QED
+
+Theorem resolve_fully_n_contract_transfer:
+  ∀p ys p' l ls pre post.
+    resolve_fully_n p ys = SOME p' ⇒
+
+    MEM l (bir_labels_of_program p) ⇒
+    ls SUBSET (set (bir_labels_of_program p)) ⇒
+
+    bir_exec_to_labels_triple p' l ls pre post ⇒
+    bir_exec_to_labels_triple p l ls pre post
+Proof
+PROVE_TAC [resolve_fully_n_simulated_termination,
+           resolve_fully_n_vars, contract_transfer]
+QED
+
+
+val _ = export_theory();
+
